Rustabelle.thy
@@ -1,9 +1,41 @@
 theory Rustabelle
-imports Main
+imports Main "~~/src/HOL/Library/While_Combinator"
 begin
 
 type_synonym ('state, 'ans) cont = "'state \<Rightarrow> 'ans"
 type_synonym ('state, 'ans) sem = "('state, 'ans) cont \<Rightarrow> ('state, 'ans) cont"
+
+abbreviation seq :: "('state, 'ans) sem \<Rightarrow> ('state, 'ans) sem \<Rightarrow> ('state, 'ans) sem" (infixl ";" 80) where
+  "seq s1 s2 \<equiv> s1 \<circ> s2"
+
+definition loop :: "('state \<Rightarrow> 'state \<times> ('state, 'ans) cont option) \<Rightarrow> 'state \<Rightarrow> 'ans" where
+  "loop l s = (let (s,s',c) = while (\<lambda>(s,s',c). c = None) (\<lambda>(s,s',c). (s',(l s'))) (s,(l s)) in the c s')"
+
+lemma loop_rule:
+  assumes "P s"
+  assumes "\<And>s s'. P s \<Longrightarrow> l s = (s',None) \<Longrightarrow> P s'" "\<And>s s' c. P s \<Longrightarrow> l s = (s',Some c) \<Longrightarrow> Q (c s')"
+  assumes "wf r" "\<And>s s'. P s \<Longrightarrow> l s = (s',None) \<Longrightarrow> (s', s) \<in> r"
+  shows "Q (loop l s)"
+sorry
+proof-
+  let ?r' = "{((s\<^sub>1,s\<^sub>1',c\<^sub>1), (s\<^sub>2,s\<^sub>2',c\<^sub>2)) | s\<^sub>1 s\<^sub>1' c\<^sub>1 s\<^sub>2 s\<^sub>2' c\<^sub>2. (s\<^sub>1,s\<^sub>2) \<in> r}"
+  have "\<And>a aa b P. \<forall>a. (\<forall>aa. (aa, a) \<in> r \<longrightarrow> (\<forall>a b. P (aa, a, b))) \<longrightarrow> (\<forall>aa b. P (a, aa, b)) \<Longrightarrow> P (a, aa, b)"
+  thm wf_def[THEN iffD1, OF assms(4), rule_format]
+  apply (rule wf_def[THEN iffD1, OF assms(4), rule_format])
+  sorry
+  have "wf ?r'"
+  apply (rule wf_def[THEN iffD2, rule_format])
+  apply (rule wf_def[THEN iffD1, OF assms(4), rule_format])
+  apply (rule wfI)
+  apply auto
+  have "\<And>s. (P \<circ> fst) s \<Longrightarrow> \<not> (case s of (s, c) \<Rightarrow> c = None) \<Longrightarrow> Q (let a = s in case a of (s, c) \<Rightarrow> the c s)"
+  by (auto intro!:assms(3))
+  show ?thesis
+  unfolding loop_def
+  term "{((s\<^sub>1,s\<^sub>1',c\<^sub>1), (s\<^sub>2,s\<^sub>2',c\<^sub>2)) | s\<^sub>1 s\<^sub>1' c\<^sub>1 s\<^sub>2 s\<^sub>2' c\<^sub>2. (s\<^sub>1,s\<^sub>2) \<in> r}"
+  apply (rule while_rule[where P="\<lambda>(s,s',c). P s \<and> (s',c) = l s" and r=?r'])
+  apply (auto simp: assms)[3]
+  apply (rule assms(4))
 
 type_synonym u32 = nat
 
@@ -15,8 +47,5 @@ abbreviation "core_iter_ops_Range_A__Iterator_next r \<equiv> case r of core_ops
 type_synonym core_option_Option = "u32 option"
 abbreviation "core_option_Option_None \<equiv> None"
 abbreviation "core_option_Option_Some \<equiv> Some"
-
-abbreviation seq :: "('state, 'ans) sem \<Rightarrow> ('state, 'ans) sem \<Rightarrow> ('state, 'ans) sem" (infixl ";" 80) where
-  "seq s1 s2 \<equiv> s1 \<circ> s2"
 
 end
