Prove.thy
@@ -1,9 +1,38 @@
 theory Prove
-imports Export
+imports Export Binomial
 begin
 
-lemma fac: "fac n = 2 * n"
-unfolding fac_def
-by simp
+(*
+lemma fac_16:
+  assumes "s 3 = core_option_Option_Some (Any_3 (core_ops_Range 2 n))"
+  shows "fac_16 (\<lambda>s. case s (Suc 0) of Some (Any_1 xa) \<Rightarrow> xa) s = fact n"
+proof-
+  have "fac_16_dom (\<lambda>a. fac_16 (\<lambda>s. case s (Suc 0) of Some (Any_1 xa) \<Rightarrow> xa) a = fact n, s)"
+  thm fac_16.domintros
+  apply (rule fac_16.domintros)
+  apply (auto split:option.splits)
+
+  
+  apply (rule fac_16.pinduct)
+*)
+
+lemma "(s(1:=1,2:=2,3:=3)) 2 = 2" by simp
+find_theorems "_(?x:=_,?y := _ )"
+lemma "(case if b then Some x else None of Some x \<Rightarrow> P x | None \<Rightarrow> Q) = P x" by simp
+lemma fac: "fac (n::u32) = fact n"
+proof-
+  let ?s = "
+     (Map.empty(0 := core_option_Option_Some (Any_0 n), Suc 0 := core_option_Option_Some (Any_1 (Suc 0)), 8 := core_option_Option_Some (Any_8 core_iter_I_IntoIterator_into_iter),
+                10 := core_option_Option_Some (Any_10 n), 9 := core_option_Option_Some (Any_9 (core_ops_Range 2 n)), 7 := core_option_Option_Some (Any_7 (core_ops_Range 2 n)),
+                3 := core_option_Option_Some (Any_3 (core_ops_Range 2 n))))"
+  show ?thesis
+  unfolding fac_def
+  apply auto
+  apply (rule loop_rule[where P="\<lambda>s. \<exists>k. s 9 = Some (Any_9 (core_ops_Range k n))"])
+  apply (auto simp: fac_16_def)[1]
+  apply (simp add: fac_16_def split:prod.splits core_ops_Range.splits)
+  apply (cases "2<n")
+  apply auto[1]
+qed
 
 end
